CoInd/M.lean
@@ -3,7 +3,6 @@ import Lean
 import CoInd.Container
 import Lean
 import Std
-import CoInd.Paco
 
 namespace Container
 variable {C:Container.{u₁}}
@@ -236,63 +235,62 @@ by
 #check M.destruct_corec
 #check M.bisim
 
-open Lean Expr Elab Term Tactic Meta Qq
-
-/-- tactic for proof by bisimulation -/
-syntax "mv_bisim" (ppSpace colGt term) (" with" (ppSpace colGt binderIdent)+)? : tactic
-
-
-elab_rules : tactic
-  | `(tactic| mv_bisim $e $[ with $ids:binderIdent*]?) => do
-    let ids : TSyntaxArray `Lean.binderIdent := ids.getD #[]
-    let idsn (n : Nat) : Name :=
-      match ids[n]? with
-      | some s =>
-        match s with
-        | `(binderIdent| $n:ident) => n.getId
-        | `(binderIdent| _) => `_
-        | _ => unreachable!
-      | none => `_
-    let idss (n : Nat) : TacticM (TSyntax `rcasesPat) := do
-      match ids[n]? with
-      | some s =>
-        match s with
-        | `(binderIdent| $n:ident) => `(rcasesPat| $n)
-        | `(binderIdent| _%$b) => `(rcasesPat| _%$b)
-        | _ => unreachable!
-      | none => `(rcasesPat| _)
-    withMainContext do
-      let e ← Tactic.elabTerm e none
-      let f ← liftMetaTacticAux fun g => do
-        let (#[fv], g) ← g.generalize #[{ expr := e }] | unreachable!
-        return (mkFVar fv, [g])
-      withMainContext do
-        let some (t, l, r) ← matchEq? (← getMainTarget) | throwError "goal is not an equality"
-        let ex ←
-          withLocalDecl (idsn 1) .default t fun v₀ =>
-            withLocalDecl (idsn 2) .default t fun v₁ => do
-              let x₀ ← mkEq v₀ l
-              let x₁ ← mkEq v₁ r
-              let xx ← mkAppM ``And #[x₀, x₁]
-              let ex₁ ← mkLambdaFVars #[f] xx
-              let ex₂ ← mkAppM ``Exists #[ex₁]
-              mkLambdaFVars #[v₀, v₁] ex₂
-        let R ← liftMetaTacticAux fun g => do
-          let g₁ ← g.define (idsn 0) (← mkArrow t (← mkArrow t (mkSort .zero))) ex
-          let (Rv, g₂) ← g₁.intro1P
-          return (mkFVar Rv, [g₂])
-        withMainContext do
-          ids[0]?.forM fun s => addLocalVarInfoForBinderIdent R s
-          let sR ← exprToSyntax R
-          evalTactic <| ← `(tactic|
-            --refine MvQPF.Cofix.bisim₂ $sR ?_ _ _ ⟨_, rfl, rfl⟩;
-            --refine Container.M.bisim $sR ?_ _ _ ⟨_, rfl, rfl⟩;
-            refine Container.M.bisim $sR ?_ _ _ ⟨_, rfl, rfl⟩;
-            rintro $(← idss 1) $(← idss 2) ⟨$(← idss 3), $(← idss 4), $(← idss 5)⟩)
-          liftMetaTactic fun g => return [← g.clear f.fvarId!]
-    for n in [6 : ids.size] do
-      let name := ids[n]!
-      logWarningAt name m!"unused name: {name}"
-#check Container.M.bisim
-
 end Container
+--open Lean Expr Elab Term Tactic Meta Qq
+
+-- syntax "m_bisim" (ppSpace colGt term) (" with" (ppSpace colGt binderIdent)+)? : tactic
+--
+--
+-- elab_rules : tactic
+--   | `(tactic| m_bisim $e $[ with $ids:binderIdent*]?) => do
+--     let ids : TSyntaxArray `Lean.binderIdent := ids.getD #[]
+--     let idsn (n : Nat) : Name :=
+--       match ids[n]? with
+--       | some s =>
+--         match s with
+--         | `(binderIdent| $n:ident) => n.getId
+--         | `(binderIdent| _) => `_
+--         | _ => unreachable!
+--       | none => `_
+--     let idss (n : Nat) : TacticM (TSyntax `rcasesPat) := do
+--       match ids[n]? with
+--       | some s =>
+--         match s with
+--         | `(binderIdent| $n:ident) => `(rcasesPat| $n)
+--         | `(binderIdent| _%$b) => `(rcasesPat| _%$b)
+--         | _ => unreachable!
+--       | none => `(rcasesPat| _)
+--     withMainContext do
+--       let e ← Tactic.elabTerm e none
+--       let f ← liftMetaTacticAux fun g => do
+--         let (#[fv], g) ← g.generalize #[{ expr := e }] | unreachable!
+--         return (mkFVar fv, [g])
+--       withMainContext do
+--         let some (t, l, r) ← matchEq? (← getMainTarget) | throwError "goal is not an equality"
+--         let ex ←
+--           withLocalDecl (idsn 1) .default t fun v₀ =>
+--             withLocalDecl (idsn 2) .default t fun v₁ => do
+--               let x₀ ← mkEq v₀ l
+--               let x₁ ← mkEq v₁ r
+--               let xx ← mkAppM ``And #[x₀, x₁]
+--               let ex₁ ← mkLambdaFVars #[f] xx
+--               let ex₂ ← mkAppM ``Exists #[ex₁]
+--               mkLambdaFVars #[v₀, v₁] ex₂
+--         let R ← liftMetaTacticAux fun g => do
+--           let g₁ ← g.define (idsn 0) (← mkArrow t (← mkArrow t (mkSort .zero))) ex
+--           let (Rv, g₂) ← g₁.intro1P
+--           return (mkFVar Rv, [g₂])
+--         withMainContext do
+--           ids[0]?.forM fun s => Meta.addLocalVarInfoForBinderIdent R s
+--           let sR ← exprToSyntax R
+--           evalTactic <| ← `(tactic|
+--             --refine MvQPF.Cofix.bisim₂ $sR ?_ _ _ ⟨_, rfl, rfl⟩;
+--             --refine Container.M.bisim $sR ?_ _ _ ⟨_, rfl, rfl⟩;
+--             refine Container.M.bisim $sR ?_ _ _ ⟨_, rfl, rfl⟩;
+--             rintro $(← idss 1) $(← idss 2) ⟨$(← idss 3), $(← idss 4), $(← idss 5)⟩)
+--           liftMetaTactic fun g => return [← g.clear f.fvarId!]
+--     for n in [6 : ids.size] do
+--       let name := ids[n]!
+--       logWarningAt name m!"unused name: {name}"
+-- #check Container.M.bisim
+
