CoInd/Tactic.lean
@@ -1,0 +1,140 @@
+
+import Qq
+import Lean
+import Std
+
+
+universe u v w
+
+open Lean Lean.Expr Lean.Meta Lean.Elab.Tactic Std
+open Qq
+
+
+namespace Tactic.Coinduction
+
+open Lean Expr Elab Term Tactic Meta Qq
+
+#check 42
+
+
+def Property.parse : List Expr → MetaM ((P: Q(Prop)) × Q($P))
+| [x] => do
+  let P ← inferType x
+  let .sort .zero ← whnf (← inferType P)
+    | throwError "{P} most be of type Prop := Sort 0 {x}"
+  return ⟨P, x⟩
+| x :: xs => do
+  let ⟨p, h⟩ ← Property.parse xs
+  let P ← inferType x
+  let .sort .zero ← whnf (← inferType P)
+    | throwError "{P} most be of type Prop := Sort 0 {x}"
+  have P : Q(Prop) := P
+  have x : Q($P) := x
+  return ⟨q($p ∧ $P), q(And.intro $h $x)⟩
+| _ => return ⟨q(True), q(True.intro)⟩
+
+
+def Exists_intro {α: Sort u} (P: α → Prop) (x: α) (h: P x) : Exists P := Exists.intro x h
+
+def matchAppN : Expr → Nat → Option (Expr × List Expr) :=
+  λ e n => (λ (x, l) => (x, l.reverse)) <$> go e n
+where
+  go : Expr → Nat → Option (Expr × List Expr)
+  | .mdata _ e, n+1 => go e (n+1)
+  | .app e a, n+1 => do
+    let (e, l) ← go e n
+    return (e, a :: l)
+  | e, 0 => some (e, [])
+  | _, _ => none
+
+def errorMessage :=
+  "A coinduction theorem must be of the form:\n" ++
+  "(p: ∀ (x₁:T₁) ... (xₙ:Tₙ) → Prop) → " ++
+  "(∀ (x₁:T₁) ... (xₙ:Tₙ), p x₁ ... xₙ → ?coindGoalFn p x₁ ... xₙ) → " ++
+  "∀ (x₁:T₁) ... (xₙ:Tₙ), p x₁ ... xₙ → ?goalFn x₁ ... xₙ" ++
+  "and the goal must be of the form" ++
+  "?goalFn, e₁, ..., eₙ" ++
+  "\n"
+
+def parseThmArgs (l: List α) : Option (α × α × List α × α) := do
+  let P :: hyp :: args := l | none
+  if args.length = 0 then none
+  let (args, [h]) := args.splitAt (args.length -1) | none
+  return (P, hyp, args, h)
+
+-- the coinduction theorem must be of the form
+-- (p: ∀ (x₁:T₁) ... (xₙ:Tₙ) → Prop) →
+-- (∀ (x₁:T₁) ... (xₙ:Tₙ), p x₁ ... xₙ → ?coindGoalFn p x₁ ... xₙ) →
+-- ∀ (x₁:T₁) ... (xₙ:Tₙ), p x₁ ... xₙ → ?goalFn x₁ ... xₙ
+-- and the goal must be of the form
+-- ?goalFn, e₁, ..., eₙ
+def parseGoal (goal: Expr) (thm: Expr) : MetaM (Expr × List Expr) := do
+  forallTelescope thm λ args goalPure => do
+    let .some (_, _, args, _) := parseThmArgs args.toList | throwError ("length error: " ++ errorMessage)
+    let .some (goalFn, _) := matchAppN goalPure args.length | throwError errorMessage
+    let .some (goalFn', exprs) := matchAppN goal args.length | throwError errorMessage
+    -- TODO: test if fvars and args are defEq
+    if not (←isDefEq goalFn goalFn') then
+      throwError "the goal and the coinduction theorem doesn't match"
+    return (goalFn, exprs)
+
+elab "coinduction" "[" hyps:term,* "]" "generalizing" "[" args:term,* "]" "using" thm:term : tactic => do
+  let thm ← Tactic.elabTerm thm none
+  have hyps : Array Term := hyps
+
+  withMainContext do
+    let mvarid ← getMainGoal
+    let goal ← getMainTarget
+    let (goalFn, exprs) ← parseGoal goal (← inferType thm)
+
+    let ⟨P, h⟩ ← Property.parse
+      <| List.reverse <| Array.toList <| ← Array.mapM (λ h => Tactic.elabTerm h none) hyps
+
+    let new_goal ← mkFreshExprMVar <| .some <| ← forallTelescope (← inferType thm) λ args goalPure => do
+      let .some (_, _, args, _) := parseThmArgs args.toList | throwError errorMessage
+      let .some (_, exprs) := matchAppN goal args.length | throwError errorMessage
+      let P ← List.foldlM (λ P (e, fv) => do
+          mkAppM `And #[← mkAppM `Eq #[e, fv], P]
+        ) P (List.zip exprs args)
+      mkForallFVars (.mk args) (←mkArrow P goalPure)
+
+    let h ← forallTelescope (← inferType thm) λ args _ => do
+      let .some (_, _, args, _) := parseThmArgs args.toList | throwError errorMessage
+      let .some (_, exprs) := matchAppN goal args.length | throwError errorMessage
+      List.foldlM (λ h e => do
+          mkAppM `And.intro #[← mkAppM `Eq.refl #[e], h]
+        ) h exprs
+
+    mvarid.assign <| .app (mkAppN new_goal <| .mk exprs) h
+    --replaceMainGoal [new_goal.mvarId!, mvarid]
+
+    let (fvars, mvarid) ← new_goal.mvarId!.generalize (← Array.mapM (λ e => do return {expr := ← Tactic.elabTerm e none}) args)
+
+    let (vars, mvarid) ← mvarid.introNP (1 + exprs.length)
+    let (vars, [init]) := vars.toList.splitAt (vars.size-1) | unreachable!
+    let init := mkFVar init
+    replaceMainGoal [mvarid]
+
+    withMainContext $ do
+      let P ← inferType init
+      let (P_closed, init_closed) ← Array.foldlM (λ (P, h) fv => do
+        if containsFVar P fv then do
+          let P_fun ← mkLambdaFVars #[mkFVar fv] P
+          let P ← mkAppM ``Exists #[←mkLambdaFVars #[mkFVar fv] P]
+          let h ← mkAppM ``Tactic.Coinduction.Exists_intro #[P_fun, mkFVar fv, h]
+          return ⟨P, h⟩
+        else return (P, h)
+      ) (P, init) (Array.reverse fvars)
+      let sP ← exprToSyntax (← mkLambdaFVars (.mk <| List.map mkFVar vars) P_closed)
+      evalTactic <| ← `(tactic|
+        apply $(←exprToSyntax thm) $sP ?_ <;> try exact $(← exprToSyntax init_closed);
+      )
+      evalTactic <| ← `(tactic|
+        clear $(←exprToSyntax init);
+      )
+      let _ ← Array.mapM (λ fv => do evalTactic <| ← `(tactic| clear $(←exprToSyntax (mkFVar fv)))) fvars
+      let _ ← List.mapM (λ fv => do evalTactic <| ← `(tactic| try clear $(←exprToSyntax (mkFVar fv)))) vars
+      return ()
+
+end Tactic.Coinduction
+
