CoInd/Utils.lean
@@ -1,7 +1,7 @@
 import CoInd.M
-import CoInd.MIdx
-import CoInd.QPF
-import CoInd.Eqns
+--import CoInd.MIdx
+--import CoInd.QPF
+--import CoInd.Eqns
 
 namespace Container
 
@@ -56,143 +56,143 @@ protected def M.casesOn' {r: C.M → Sort w} (x: C.M) (f: ∀ x: C.Obj C.M, r (M
 end Container
 
 
-namespace IContainer
-
-variable {I:Type u₀}
-variable {C:IContainer.{u₀} I}
-
-#check Map
-#check M.destruct
-
-def M.construct.automaton (i:I) : C.Obj (M C) i → C.Obj (C.Obj (M C)) i := Map (@destruct I C)
-
-def M.construct {i:I} (x₀: C.Obj (M C) i) : M C i :=
-  M.corec M.construct.automaton x₀
-
-def M.construct_def {i:I} : @construct I C i = corec (@construct.automaton I C) := by rfl
-
-
-theorem M.construct_destruct {i:I} (x:M C i) : construct (destruct x) = x :=
-by
-  let R i (x y: M C i) := x = construct (destruct y)
-  apply bisim R
-  . intro i x y h₀
-    have h₀ := congrArg destruct h₀
-    cases h₁:destruct y
-    case mk node k₂ =>
-      rw [h₁] at h₀
-      simp only [construct, destruct_corec, Map] at h₀
-      simp only [construct.automaton, Map] at h₀
-      exists node
-      exists λ (x:B C i node) => construct <| destruct <| k₂ x
-      exists k₂
-      constructor
-      . exact h₀
-      . constructor
-        . rfl
-        . intro i
-          rfl
-  . rfl
-
-
-def M.destruct_construct {i:I} : ∀ x: C.Obj (M C) i, destruct (construct x) = x :=
-by
-  intro ⟨n, k⟩
-  --simp only [construct, construct.automaton]
-  have : (destruct (construct ⟨n, k⟩)).fst = n := by
-    rfl
-
-  simp only [construct]
-  rw [destruct_corec construct.automaton ⟨n, k⟩]
-  simp only [←construct_def]
-  simp only [construct.automaton, Map]
-
-  have : (λ x : B C i n => construct <| destruct <| k x) = k := by
-    funext x
-    simp only [Function.comp]
-    rw [M.construct_destruct]
-
-  rw [this]
-
-
-attribute [eqns QPF.M.construct_destruct] M.construct
-attribute [eqns QPF.M.destruct_construct QPF.M.destruct_corec] M.destruct
-
-#check M.construct
-#check M.construct_destruct
-#check M.destruct_construct
-
-#check Functor
-
-end IContainer
-
-
-namespace QPF
-
-variable {F:Type u₁ → Type u₁} [inst:QPF F]
-def M.construct.automaton : F (M F) → F (F <| M F) := Functor.map M.destruct
-
-def M.construct (x₀: F (M F)) : M F :=
-  M.corec M.construct.automaton x₀
-
-#check M.corec
-#check M.construct
-def M.construct_def : construct = corec (@construct.automaton F _) := by rfl
-
-
-theorem M.construct_destruct (x:M F) : construct (destruct x) = x :=
-by
-  let R (x y: M F) := x = construct (destruct y)
-  apply bisim R
-  . intro x y h₀
-    have h₀ := congrArg destruct h₀
-    --rw [h₀]
-    simp [liftr]
-    simp only [construct, destruct_corec, construct.automaton] at h₀
-    exists Functor.map (λ a => ⟨⟨construct <| destruct a, a⟩, by simp⟩) (destruct y)
-    rw [h₀]
-    constructor
-    . simp only [←QPF.map_comp]
-      rfl
-    . rw [←QPF.M.map_comp]
-      have : inst.map id (destruct y) = destruct y := by rw [QPF.map_id]
-      apply Eq.trans _ this
-      apply congrFun
-      funext _
-      rfl
-  . rfl
-
-def M.destruct_construct : ∀ x: F (M F), destruct (construct x) = x :=
-by
-  intro x
-
-  simp only [construct]
-  rw [destruct_corec]
-  conv =>
-    lhs
-    lhs
-    rw [←@construct_def F]
-  simp only [construct.automaton]
-  rw [←map_comp]
-  apply Eq.trans _ (QPF.map_id x)
-  conv =>
-    lhs
-    lhs
-    intro x
-    simp only [Function.comp, construct_destruct]
-
-
-attribute [eqns QPF.M.construct_destruct] M.construct
-attribute [eqns QPF.M.destruct_construct QPF.M.destruct_corec] M.destruct
-
-#check M.construct
-#check M.construct_destruct
-#check M.destruct_construct
-
-example : ∀ x:M F, M.construct (M.destruct x) = x := by
-  intro x
-  simp [M.construct]
-
-
-
-end QPF
+--namespace IContainer
+--
+--variable {I:Type u₀}
+--variable {C:IContainer.{u₀} I}
+--
+--#check Map
+--#check M.destruct
+--
+--def M.construct.automaton (i:I) : C.Obj (M C) i → C.Obj (C.Obj (M C)) i := Map (@destruct I C)
+--
+--def M.construct {i:I} (x₀: C.Obj (M C) i) : M C i :=
+--  M.corec M.construct.automaton x₀
+--
+--def M.construct_def {i:I} : @construct I C i = corec (@construct.automaton I C) := by rfl
+--
+--
+--theorem M.construct_destruct {i:I} (x:M C i) : construct (destruct x) = x :=
+--by
+--  let R i (x y: M C i) := x = construct (destruct y)
+--  apply bisim R
+--  . intro i x y h₀
+--    have h₀ := congrArg destruct h₀
+--    cases h₁:destruct y
+--    case mk node k₂ =>
+--      rw [h₁] at h₀
+--      simp only [construct, destruct_corec, Map] at h₀
+--      simp only [construct.automaton, Map] at h₀
+--      exists node
+--      exists λ (x:B C i node) => construct <| destruct <| k₂ x
+--      exists k₂
+--      constructor
+--      . exact h₀
+--      . constructor
+--        . rfl
+--        . intro i
+--          rfl
+--  . rfl
+--
+--
+--def M.destruct_construct {i:I} : ∀ x: C.Obj (M C) i, destruct (construct x) = x :=
+--by
+--  intro ⟨n, k⟩
+--  --simp only [construct, construct.automaton]
+--  have : (destruct (construct ⟨n, k⟩)).fst = n := by
+--    rfl
+--
+--  simp only [construct]
+--  rw [destruct_corec construct.automaton ⟨n, k⟩]
+--  simp only [←construct_def]
+--  simp only [construct.automaton, Map]
+--
+--  have : (λ x : B C i n => construct <| destruct <| k x) = k := by
+--    funext x
+--    simp only [Function.comp]
+--    rw [M.construct_destruct]
+--
+--  rw [this]
+--
+--
+--attribute [eqns QPF.M.construct_destruct] M.construct
+--attribute [eqns QPF.M.destruct_construct QPF.M.destruct_corec] M.destruct
+--
+--#check M.construct
+--#check M.construct_destruct
+--#check M.destruct_construct
+--
+--#check Functor
+--
+--end IContainer
+--
+--
+--namespace QPF
+--
+--variable {F:Type u₁ → Type u₁} [inst:QPF F]
+--def M.construct.automaton : F (M F) → F (F <| M F) := Functor.map M.destruct
+--
+--def M.construct (x₀: F (M F)) : M F :=
+--  M.corec M.construct.automaton x₀
+--
+--#check M.corec
+--#check M.construct
+--def M.construct_def : construct = corec (@construct.automaton F _) := by rfl
+--
+--
+--theorem M.construct_destruct (x:M F) : construct (destruct x) = x :=
+--by
+--  let R (x y: M F) := x = construct (destruct y)
+--  apply bisim R
+--  . intro x y h₀
+--    have h₀ := congrArg destruct h₀
+--    --rw [h₀]
+--    simp [liftr]
+--    simp only [construct, destruct_corec, construct.automaton] at h₀
+--    exists Functor.map (λ a => ⟨⟨construct <| destruct a, a⟩, by simp⟩) (destruct y)
+--    rw [h₀]
+--    constructor
+--    . simp only [←QPF.map_comp]
+--      rfl
+--    . rw [←QPF.M.map_comp]
+--      have : inst.map id (destruct y) = destruct y := by rw [QPF.map_id]
+--      apply Eq.trans _ this
+--      apply congrFun
+--      funext _
+--      rfl
+--  . rfl
+--
+--def M.destruct_construct : ∀ x: F (M F), destruct (construct x) = x :=
+--by
+--  intro x
+--
+--  simp only [construct]
+--  rw [destruct_corec]
+--  conv =>
+--    lhs
+--    lhs
+--    rw [←@construct_def F]
+--  simp only [construct.automaton]
+--  rw [←map_comp]
+--  apply Eq.trans _ (QPF.map_id x)
+--  conv =>
+--    lhs
+--    lhs
+--    intro x
+--    simp only [Function.comp, construct_destruct]
+--
+--
+--attribute [eqns QPF.M.construct_destruct] M.construct
+--attribute [eqns QPF.M.destruct_construct QPF.M.destruct_corec] M.destruct
+--
+--#check M.construct
+--#check M.construct_destruct
+--#check M.destruct_construct
+--
+--example : ∀ x:M F, M.construct (M.destruct x) = x := by
+--  intro x
+--  simp [M.construct]
+--
+--
+--
+--end QPF
